Hoare logic formalization proved up to seq rule

examples/hoare_logic/imp/imp_Imp_eval_subst_2.v
@@ -100,11 +100,6 @@ Inductive many_steps : (map ident Z) -> stmt -> (map ident Z)
       ident Z)) (i1:stmt) (i2:stmt) (i3:stmt), (one_step s1 i1 s2 i2) ->
       ((many_steps s2 i2 s3 i3) -> (many_steps s1 i1 s3 i3)).
 
-Axiom many_steps_seq_rec : forall (s1:(map ident Z)) (s3:(map ident Z))
-  (i:stmt) (i3:stmt), (many_steps s1 i s3 i3) -> ((i3 = Sskip) ->
-  forall (i1:stmt) (i2:stmt), (i = (Sseq i1 i2)) -> exists s2:(map ident Z),
-  (many_steps s1 i1 s2 Sskip) /\ (many_steps s2 i2 s3 Sskip)).
-
 Axiom many_steps_seq : forall (s1:(map ident Z)) (s3:(map ident Z)) (i1:stmt)
   (i2:stmt), (many_steps s1 (Sseq i1 i2) s3 Sskip) -> exists s2:(map ident
   Z), (many_steps s1 i1 s2 Sskip) /\ (many_steps s2 i2 s3 Sskip).
@@ -138,32 +133,16 @@ Definition subst(f:fmla) (x:ident) (t:expr): fmla :=
   | (Fterm e) => (Fterm (subst_expr e x t))
   end.
 
-Axiom eval_subst : forall (s:(map ident Z)) (f:fmla) (x:ident) (t:expr),
-  (eval_fmla s (subst f x t)) -> (eval_fmla (set s x (eval_expr s t)) f).
-
-Definition valid_triple(p:fmla) (i:stmt) (q:fmla): Prop := forall (s:(map
-  ident Z)), (eval_fmla s p) -> forall (sqt:(map ident Z)), (many_steps s i
-  sqt Sskip) -> (eval_fmla sqt q).
-
 (* YOU MAY EDIT THE CONTEXT BELOW *)
 
 (* DO NOT EDIT BELOW *)
 
-Theorem assign_rule : forall (q:fmla) (x:ident) (e:expr),
-  (valid_triple (subst q x e) (Sassign x e) q).
+Theorem eval_subst : forall (s:(map ident Z)) (f:fmla) (x:ident) (t:expr),
+  (eval_fmla s (subst f x t)) -> (eval_fmla (set s x (eval_expr s t)) f).
 (* YOU MAY EDIT THE PROOF BELOW *)
-intros q x e.
-unfold valid_triple.
-intros s Pre s' Hred.
-inversion Hred; subst.
-inversion H; subst.
-inversion H0; subst.
-(* normal case *)
-clear H Hred H0.
-apply eval_subst; auto.
-
-(* absurd case *)
-inversion H1.
+induction f; unfold eval_fmla, subst in *.
+intros x t H.
+rewrite <- eval_subst_expr; auto.
 Qed.
 (* DO NOT EDIT BELOW *)
 
